Add many more finite set examples
Some of them are admitted at the moment, but they're all listed.
(Finished 11/15 examples.)

Also work around the extremely annoying
    Anomaly: Uncaught exception Invalid_argument("decomp_pointwise").
    Please report.
I hope I didn't break anything by guarding some [setoid_rewrite]s in
Computation/Monad.v; I didn't test super-thoroughly.

src/FiniteSetADTs/FiniteSetADT.v
@@ -11,12 +11,66 @@ Module Type BedrockWordT.
   Axiom W : Type.
   Axiom wzero : W.
   Axiom wplus : W -> W -> W.
+  Axiom weq : W -> W -> bool.
+  Axiom wlt : W -> W -> bool.
+  Axiom weq_iff : forall x y, x = y <-> weq x y = true.
+  Axiom wlt_irrefl : forall x, wlt x x = false.
+  Axiom wlt_trans : forall x y z, wlt x y = true -> wlt y z = true -> wlt x z = true.
+  Axiom wle_antisym : forall x y, wlt x y = false -> wlt y x = false -> x = y.
+  Axiom wle_asym : forall x y, wlt x y = true -> wlt y x = false.
 End BedrockWordT.
 
 Module Export BedrockWord : BedrockWordT.
   Definition W := nat.
   Definition wzero := 0.
   Definition wplus := plus.
+  Fixpoint weq (x : nat) (y : nat) : bool :=
+    match x, y with
+      | 0, 0 => true
+      | 0, S _ => false
+      | S _, 0 => false
+      | S x', S y' => weq x' y'
+    end.
+  Fixpoint wlt (x : nat) (y : nat) : bool :=
+    match x, y with
+      | 0, 0 => false
+      | 0, S _ => true
+      | S _, 0 => false
+      | S x', S y' => wlt x' y'
+    end.
+  Lemma weq_iff x : forall y, x = y <-> weq x y = true.
+  Proof.
+    induction x; intro y; destruct y;
+    split; simpl;
+    intro H;
+    first [ reflexivity
+          | exfalso; revert H; clear; intro H; abstract inversion H
+          | apply (f_equal pred) in H; simpl in H; apply IHx; assumption
+          | apply (f_equal S); apply IHx; assumption ].
+  Qed.
+  Lemma wlt_irrefl x : wlt x x = false.
+  Proof.
+    induction x; simpl; congruence.
+  Qed.
+  Lemma wlt_trans x : forall y z, wlt x y = true -> wlt y z = true -> wlt x z = true.
+  Proof.
+    induction x; intros [|?] [|?]; simpl; intros;
+    try congruence.
+    eapply IHx; eassumption.
+  Qed.
+  Lemma wle_antisym x : forall y, wlt x y = false -> wlt y x = false -> x = y.
+  Proof.
+    induction x; intros [|?]; intros; simpl in *;
+    try congruence.
+    apply f_equal.
+    eapply IHx; eassumption.
+  Qed.
+  Lemma wle_asym x : forall y, wlt x y = true -> wlt y x = false.
+  Proof.
+    induction x; intros [|?]; simpl; intros;
+    try congruence.
+    apply IHx; assumption.
+  Qed.
 End BedrockWord.
 
 (** TODO: Test: Do we get a speedup if we replace these definitions
@@ -104,3 +158,20 @@ Lemma Ensemble_fold_right_simpl' {A B} f b S
 Proof.
   exact (Ensemble_fold_right_simpl f b S).
 Qed.
+
+Definition list_filter_pred {T} (P : T -> Prop) (ls : list T)
+  := List.fold_right
+       (fun (a : T) (xs : Comp (list T)) =>
+          (xs' <- xs;
+           b <- { b : bool | b = true <-> P a };
+           ret (if b then a::xs' else xs')))
+       (ret nil)
+       ls.
+
+Definition filter_pred {T} (P : T -> Prop) (S : Ensemble T)
+  := fold_right
+       (fun (a : T) (xs : list T) =>
+          (b <- { b : bool | b = true <-> P a };
+           ret (if b then a::xs else xs)))
+       (ret nil)
+       S.
